chore: remove `Mutable` and fix `UnionFind` API
Remove `Mutable`, as we could not find a design that supports `UnionFind` over polymorphic index types without running into the [polymorphic references](https://counterexamples.org/polymorphic-references.html) problem.

cpp/ffi.cpp
@@ -1,6 +1,0 @@
-#include <lean/lean.h>
-
-extern "C" LEAN_EXPORT b_lean_obj_res lean_Mutable_set(b_lean_obj_arg ref, lean_obj_arg a, b_lean_obj_arg b) {
-    lean_st_ref_set(ref, a);
-    return b;
-}
